---
layout: post
title: HDU-5780 gcd
---

First notice that $\gcd(x^a-1, x^b-1) = x^{\gcd(a,b)}-1$.

Define $C(d)$ as number of pairs that $\gcd(a, b)=d$ and $1\le a, b \le n$.
We have 

$$
C(d) = 2 \sum\limits_{i=1}^{\frac {n}{d}} \phi(i) - 1
$$

and the answer we are looking for is

$$
\text{ans} = \sum\limits_{d=1}^{n} C(d) \cdot (x^d - 1)
$$

Define $D(t) = 2\sum\limits_{i=1}^{t} \phi(i) - 1$, we have

$$
\text{ans} = \sum\limits_{d=1}^{n} D(\lfloor \frac {n}{d} \rfloor) \cdot (x^d - 1)
$$

This summation can be done in $O(\sqrt{N})$ time since the partial sum of $x^d-1$ is
easy to calculate.
